examples/sgx/Ast.fst
@@ -1,12 +1,16 @@
 module Ast
 
 open FStar.UInt32
+open FStar.UInt64
+
+open Helper
+
 let u32 = UInt32.t
+let u64 = UInt64.t
 
 type exp =
  |Reg of string
- |Constant of u32
- |Function of string
+ |Constant of u64
 
 type stmt = 
  |Store of exp * exp
@@ -20,3 +24,10 @@ type stmt =
  |Assert
 
 type program = stmt
+
+type sgxmem = 
+| Register of string
+| Memory of u64
+
+val lookup: (sgxmem->u64)->sgxmem -> u64
+val extend: (sgxmem -> u64)->sgxmem->u64 ->(sgxmem->u64)
