examples/sgx/X86Interpreter.fst
@@ -2,28 +2,41 @@ module X86Interpreter
 
 open FStar.Mul
 open FStar.Ghost
-open FStar.HyperStack
 open FStar.HST
 open FStar.Int.Cast
-open FStar.UInt8
-open FStar.UInt32
+open FStar.UInt64
 open FStar.Buffer
 open Ast
 open FStar.List
 
-module HH = FStar.HyperHeap
-module HS = FStar.HyperStack
+exception Halt
 
-let u32 = UInt32.t
-let u8 = UInt8.t
-let uint32s = buffer u32
-let bytes = buffer u8
+(* Fix these definitions *)
+let lookup sgxenv key =  sgxenv key
+let extend sgxenv key value = sgxenv
+let get_register_string r = 
+	begin match r with
+	|Reg rs -> rs
+	|_ -> raise Halt
+	end 
 
-let rec interpret program = begin match program with
-  | Skip -> IO.print_string "This a hello from Skip\n" 
-  | Store (ea, ed)
-  | Load  (ea, ed)-> IO.print_string "This a hello from Load/Store \n"
-  | Seq li -> iter interpret li 
-  | _   -> IO.print_string "Unsupported instruction *\n"
+val interpret_exp: exp -> (sgxmem->u64) -> u64
+let interpret_exp e (sgxenv: sgxmem->u64) = begin match e with
+ | Reg r -> lookup sgxenv (Register r)
+ | Constant u -> u
+end
+
+val interpret: stmt -> (sgxmem->u64) -> (sgxmem->u64)
+let rec interpret progstmt (sgxenv: sgxmem->u64) = begin match progstmt with
+  | Skip -> sgxenv 
+  | Store(ea, ed)-> let lea = interpret_exp ea sgxenv in
+		     let leb = interpret_exp ed sgxenv  in
+		     extend sgxenv (Memory lea) leb  
+  | Load(r, ea)-> let lea = interpret_exp ea sgxenv in
+		    let v = lookup sgxenv (Memory lea) in
+		    let rs = get_register_string r in
+		    extend sgxenv (Register rs) v  
+  | Seq(li) -> fold_left (fun sgxenv elem ->interpret elem sgxenv) sgxenv li 
+  | _   -> sgxenv
 end
 
