examples/sgx/Helper.fst
@@ -1,0 +1,6 @@
+module Helper
+open FStar.UInt64
+
+let int_of_string s = of_string s
+
+
